src/Layers/CryptoLayer/Definitions.v
@@ -33,29 +33,41 @@ Definition encryptionmap := @mem value value_dec (key * value).
     forall T, oracle' ->  state' -> prog' T -> @Result state' T -> Prop :=
 
   | ExecHash : 
-      forall em hm h v,
+      forall s h v,
+        let kl := fst (fst s) in
+        let em := snd (fst s) in
+        let hm := snd s in
         let hv := hash_function h v in
         consistent hm hv (h, v) ->
-        exec' [Cont] (em, hm) (Hash h v) (Finished (em, (upd hm hv (h, v))) hv)
+        exec' [Cont] s (Hash h v) (Finished (kl, em, (upd hm hv (h, v))) hv)
              
   | ExecEncrypt : 
-      forall kl em hm k v,
+      forall s k v,
+        let kl := fst (fst s) in
+        let em := snd (fst s) in
+        let hm := snd s in
         let ev := encrypt k v in
         consistent em ev (k, v) ->
-        exec' [Cont] (kl, em, hm) (Encrypt k v) (Finished (kl, (upd em ev (k, v)), hm) ev)
+        exec' [Cont] s (Encrypt k v) (Finished (kl, (upd em ev (k, v)), hm) ev)
 
   | ExecDecrypt : 
-      forall kl em hm ev k v,
+      forall s ev k v,
+        let kl := fst (fst s) in
+        let em := snd (fst s) in
+        let hm := snd s in
         ev = encrypt k v ->
         em ev = Some (k, v) ->
-        exec' [Cont] (kl, em, hm) (Decrypt k ev) (Finished (kl, em, hm) v)
+        exec' [Cont] s (Decrypt k ev) (Finished s v)
 
   | ExecGetKey : 
-      forall vl kl em hm k,
+      forall vl s k,
+        let kl := fst (fst s) in
+        let em := snd (fst s) in
+        let hm := snd s in
         ~In k kl ->
         consistent_with_upds em
              (map (encrypt k) vl) (map (fun v => (k, v)) vl) ->
-        exec' [Key k] (kl, em, hm) (GetKey vl) (Finished ((k::kl), em, hm) k)
+        exec' [Key k] s (GetKey vl) (Finished ((k::kl), em, hm) k)
  
   | ExecCrash :
       forall T d (p: prog' T),
@@ -67,15 +79,19 @@ Definition encryptionmap := @mem value value_dec (key * value).
     match p in prog' T' return (T' -> state' -> Prop) -> oracle' -> state' -> Prop with
     | Hash h v =>
       fun Q o s =>
-        let '(em, hm) := s in
-        o = [Cont] /\
+        let kl := fst (fst s) in
+        let em := snd (fst s) in
+        let hm := snd s in
         let hv := hash_function h v in
+        o = [Cont] /\
         consistent hm hv (h, v) /\
-        Q hv (em, (upd hm hv (h, v)))
+        Q hv (kl, em, (upd hm hv (h, v)))
 
     | Encrypt k v => 
       fun Q o s =>
-        let '(kl, em, hm) := s in
+        let kl := fst (fst s) in
+        let em := snd (fst s) in
+        let hm := snd s in
         let ev := encrypt k v in
         o = [Cont] /\
         consistent em ev (k, v) /\
@@ -83,7 +99,9 @@ Definition encryptionmap := @mem value value_dec (key * value).
 
     | Decrypt k ev => 
       fun Q o s =>
-        let '(kl, em, hm) := s in
+        let kl := fst (fst s) in
+        let em := snd (fst s) in
+        let hm := snd s in
         exists v,
           o = [Cont] /\
           ev = encrypt k v /\
@@ -92,17 +110,72 @@ Definition encryptionmap := @mem value value_dec (key * value).
           
     | GetKey vl =>
       fun Q o s =>
-        let '(kl, em, hm) := s in
-        (exists k,
-           o = [Key k] /\
-           ~In k kl /\
-           consistent_with_upds em (map (encrypt k) vl) (map (fun v => (k,v)) vl) /\
-           Q k ((k::kl), em, hm))
+        let kl := fst (fst s) in
+        let em := snd (fst s) in
+        let hm := snd s in
+        exists k,
+          o = [Key k] /\
+          ~In k kl /\
+          consistent_with_upds em (map (encrypt k) vl) (map (fun v => (k,v)) vl) /\
+          Q k ((k::kl), em, hm)
     end.
 
 
   Definition weakest_crash_precondition' T (p: prog' T) :=
     fun Q o (s: state') => o = [Crash] /\ Q s.
+
+  Definition strongest_postcondition' T (p: prog' T) :=
+    match p in prog' T' return (oracle' -> state' -> Prop) -> T' -> state' -> Prop with
+    | Hash h v =>
+      fun P t s' =>
+        exists s,
+        let kl := fst (fst s) in
+        let em := snd (fst s) in
+        let hm := snd s in
+        let hv := hash_function h v in
+        P [Cont] s /\
+        consistent hm hv (h, v) /\
+        t = hv /\
+        s' = (kl, em, (upd hm hv (h, v)))
+               
+    | Encrypt k v => 
+      fun P t s' =>
+        exists s,
+        let kl := fst (fst s) in
+        let em := snd (fst s) in
+        let hm := snd s in
+        let ev := encrypt k v in
+        P [Cont] s /\
+        consistent em ev (k, v) /\
+        t = ev /\
+        s' = (kl, (upd em ev (k, v)), hm)
+
+    | Decrypt k ev => 
+      fun P t s' =>
+        exists s v,
+        let kl := fst (fst s) in
+        let em := snd (fst s) in
+        let hm := snd s in
+        P [Cont] s /\
+        ev = encrypt k v /\
+        em ev = Some (k, v) /\
+        t = v /\ s' = s
+          
+    | GetKey vl =>
+      fun P t s' =>
+        exists s k,
+        let kl := fst (fst s) in
+        let em := snd (fst s) in
+        let hm := snd s in
+        P [Key k] s /\
+        ~In k kl /\
+        consistent_with_upds em (map (encrypt k) vl) (map (fun v => (k,v)) vl) /\
+        t = k /\
+        s' = ((k::kl), em, hm)
+    end.
+
+  Definition strongest_crash_postcondition' T (p: prog' T) :=
+    fun (P: oracle' -> state' -> Prop) s' => P [Crash] s'.
 
   Theorem exec_deterministic_wrt_oracle' :
     forall o s T (p: prog' T) ret1 ret2,
@@ -118,6 +191,29 @@ Definition encryptionmap := @mem value value_dec (key * value).
       end; eauto.
   Qed.
 
+  Theorem sp_complete':
+    forall T (p: prog' T) P (Q: _ -> _ -> Prop),
+      (forall t s', strongest_postcondition' p P t s' -> Q t s') <->
+      (forall o s s' t, P o s -> exec' o s p (Finished s' t) -> Q t s').
+  Proof.
+    intros; destruct p; simpl; eauto;
+    split; intros;
+    try inversion H1; cleanup;
+    eapply H; eauto;
+    do 2 eexists; eauto.    
+  Qed.
+
+  Theorem scp_complete':
+    forall T (p: prog' T) P (Q:  _ -> Prop),
+      (forall s', strongest_crash_postcondition' p P s' -> Q s') <->
+      (forall o s s', P o s -> exec' o s p (Crashed s') -> Q s').
+  Proof.
+    intros; destruct p; simpl; eauto;
+    split; intros;
+    try inversion H1; cleanup;
+    eapply H; eauto.
+  Qed.
+
   Theorem wp_complete':
     forall T (p: prog' T) H Q,
       (forall o s, H o s -> weakest_precondition' p Q o s) <->
@@ -127,7 +223,7 @@ Definition encryptionmap := @mem value value_dec (key * value).
     split; intros;
     specialize H0 with (1:= X);
     cleanup; eauto;
-    inversion H0; cleanup; eauto.
+    inversion H0; cleanup; eauto.    
   Qed.
   
   Theorem wcp_complete':
@@ -151,14 +247,16 @@ Definition encryptionmap := @mem value value_dec (key * value).
       exec'
       weakest_precondition'
       weakest_crash_precondition'
+      strongest_postcondition'
+      strongest_crash_postcondition'
       wp_complete'
       wcp_complete'
+      sp_complete'
+      scp_complete'
       exec_deterministic_wrt_oracle'.
   
   Definition CryptoLang := Build_Language CryptoOperation.
   Definition CryptoHL := Build_HoareLogic CryptoLang.
-
-
 
 Notation "| p |" := (Op CryptoOperation p)(at level 60).
 Notation "x <-| p1 ; p2" := (Bind (Op CryptoOperation p1) (fun x => p2))(right associativity, at level 60).
